Change binary code definition to better match maths

theories/Codes.v
@@ -1,9 +1,12 @@
 Require Import ssreflect ssrbool ssrfun.
 From HB Require Import structures.
-From mathcomp Require Import ssrnat eqtype choice div seq preorder.
+From mathcomp Require Import
+  ssrnat eqtype choice div seq preorder order path
+  zify.
 From Thompson Require Import PrefixOrder.
 
 Import Order.PreorderTheory.
+Import Order.POrderTheory.
 
 Open Scope order_scope.
 
@@ -24,25 +27,39 @@ Open Scope order_scope.
    x >< y <-> x and y are incomparable
    *)
 
-(* TODO(reiniscirpons): Maybe do sets? *)
-Definition binary_code := seq binary_word.
+(* NOTE(reiniscirpons):
+   We require a binary_code to be a set. We implement
+   this by requiring that a binary code be sorted with
+   respect to the lexicographic order on sequences.
+   Since we use the non-strict order <=%O below, it
+   follows that we actually allow for multisets, which
+   may be useful in the future. *)
+Definition binary_code (code: seq binary_word) :=
+  sorted (<=%O) (code: seq (seqlexi bool)).
 
 (* TODO(reiniscirpons): Explicitly mention prefix codes are finite
    in this development *)
-Fixpoint prefix_code (code: binary_code): bool :=
-  match code with
-  | nil => true
-  | word::code' =>
-    (all (fun word' => word' >< word) code') &&
-    (prefix_code code')
-  end.
+(*Fixpoint prefix_code (code: binary_code): bool :=*)
+(*  match code with*)
+(*  | nil => true*)
+(*  | word::code' =>*)
+(*    (all (fun word' => word' >< word) code') &&*)
+(*    (prefix_code code')*)
+(*  end.*)
+
+Definition prefix_code (code: seq binary_word): bool :=
+  binary_code code &&
+  pairwise (fun x y => (x >< y)) code.
+
 
 (* The following lemma establishes that the `prefix_code` function
-    coincides with the mathematical definition of a prefix code. *)
+   coincides with the mathematical definition of a prefix code.
+   Note we implement the set condition by requiring that it
+   is strictly sorted with respect to the lexicographic order. *)
 Lemma prefix_codeP: forall code,
   reflect
-    (uniq code /\
-      (forall word1 word2,
+    (sorted (<%O) (code: seq (seqlexi bool)) /\
+      (forall (word1 word2: binary_word),
         word1 \in code ->
         word2 \in code ->
         word1 >=< word2 ->
@@ -50,44 +67,80 @@ Lemma prefix_codeP: forall code,
     (prefix_code code).
 Proof.
   move => code; apply (iffP idP) => /= [|[]].
-  - elim: code => /= [//|word code IH /andP [/allP Hcomp /IH {IH} [-> H]]].
-    split => [|word1 word2].
-  -- apply /andP; split => [|//].
-     apply /memPn => /= word' /Hcomp.
-     apply contra => /eqP ->.
-     Locate comparablexx.
-     by exact: comparablexx.
+  - rewrite /prefix_code =>
+      /andP [/sortedP Hsort Hcomp]; split.
+  -- apply /(sortedP [::]) => i Hi.
+     move: (Hsort [::] i Hi).
+     rewrite le_eqVlt => /orP [/eqP H|//].
+     exfalso.
+     enough (Hfalso: nth [::] code i >< nth [::] code i.+1);
+       first by move/incomparable_eqF/eqP: Hfalso; rewrite H.
+     move/pairwiseP in Hcomp.
+     apply Hcomp => [|//|//];
+       (* TODO(reiniscirpons): Why does by lia fail here !?*)
+     enough (Hi': (i < size code)%N) => [//|].
+     by apply ltn_trans with i.+1.
+
+  - elim: code Hcomp {Hsort} => /=
+      [//|word code IH /andP [/allP Hcomp /IH {IH} H] word1 word2].
   -- rewrite !in_cons => /orP [/eqP ->|H1] /orP [/eqP ->|H2] //.
-  --- by rewrite comparable_sym; move: H2 => /Hcomp /negP.
-  --- by move: H1 => /Hcomp /negP.
+  --- by move: H2 => /Hcomp /negP.
+  --- by move: H1 => /Hcomp /negP; rewrite comparable_sym.
   --- by move => H3; apply H.
-  - elim: code => /= [//|word code IH /andP [/memPn Hword Huniq] H].
+  - elim: code => [//|word code IH Hsort Hcomp].
     apply /andP; split.
-  -- apply /allP => word' Hword'.
-     apply /negP => Hcomp.
-     enough (Heq: word = word').
-  --- move: (Hword word' Hword') => /eqP; by rewrite Heq.
-  --- apply H.
-  ---- by rewrite in_cons eq_refl.
-  ---- by rewrite in_cons Hword'; apply /orP; right.
-  ---- by rewrite comparable_sym.
-  -- apply IH => [//|word1 word2 H1 H2 Hcomp].
-     apply H => [||//]; rewrite in_cons; apply /orP; by right.
+  -- apply /(sortedP [::]) => i Hi.
+     rewrite le_eqVlt; apply /orP; right.
+     move/sortedP in Hsort.
+     by apply Hsort.
+
+  -- enough (H: prefix_code code).
+  --- move/andP: H => /= [_ ->].
+      apply /andP; split => [|//].
+      apply/allP => x Hx; apply /negP => Hwx.
+      enough (Hfalso: word = x).
+  ---- move: Hsort; rewrite sorted_pairwise /=;
+         last by exact: lt_trans.
+       move/andP => [/allP H];
+       by move: (H x Hx); rewrite Hfalso ltxx.
+  ---- apply Hcomp => [||//];
+       rewrite in_cons; apply/orP.
+  ----- by left.
+  ----- by right.
+  -- apply IH;
+       first by move/(drop_sorted 1): Hsort => /=; rewrite drop0.
+     move => word1 word2 H1 H2 H12; apply Hcomp => [||//];
+     by rewrite in_cons; apply/orP; right.
 Qed.
 
-Definition prepend (letter: bool) (code: binary_code): binary_code :=
-  [seq letter::word | word <- code].
+Definition prepend (letter: bool) (code: seq binary_word):
+  seq binary_word :=
+    [seq letter::word | word <- code].
+
+Lemma prepend_cons: forall letter word code,
+  prepend letter (word::code) = (letter::word)::(prepend letter code).
+Proof. done. Qed.
+
+Lemma binary_code_prepend: forall letter code,
+  binary_code code -> binary_code (prepend letter code).
+Proof.
+  move => letter; elim =>
+    [//|word1 [//|word2 code]] /= IH /andP [H /IH ->].
+  by rewrite eqhead_lexiE H.
+Qed.
 
 Lemma prefix_code_prepend: forall letter code,
   prefix_code code -> prefix_code (prepend letter code).
 Proof.
-  move => letter; elim => [//|word code'] /= IH /andP [/allP H /IH H'].
+  move => letter code;
+  rewrite /prefix_code => /andP [/(binary_code_prepend letter)] -> /=.
+  elim: code => [//|word code /= IH /andP [/allP H /IH ->]].
   apply /andP; split => [|//].
-  apply /allP => word' /mapP /= [word'' /H H'' ->].
-  by rewrite seqprefix_comparable_cons eq_refl /=.
+  apply /allP => x /mapP [y /H Hy ->].
+  by rewrite seqprefix_comparable_cons eq_refl.
 Qed.
 
-Lemma prepend_uniq: forall (letter: bool) (code: binary_code),
+Lemma prepend_uniq: forall (letter: bool) (code: seq binary_word),
   uniq code -> uniq (prepend letter code).
 Proof.
   move => letter; elim => [//|word code IH /= /andP [Hw /IH ->]].
@@ -97,16 +150,27 @@ Proof.
   by move/negP: Hw.
 Qed.
 
+Lemma binary_code_behead: forall {word code},
+  binary_code (word::code) -> binary_code code.
+Proof.
+  by move => word1 [//|word2 code /= /andP [_ ->]].
+Qed.
+
 Lemma prefix_code_behead: forall word code,
   prefix_code (word::code) -> prefix_code code.
 Proof.
-  by move => word code /= /andP [].
+  rewrite /prefix_code.
+  by move => word code /= /andP
+    [/binary_code_behead -> /= /andP [_ ->]].
 Qed.
 
 Lemma prefix_code_cons_nil: forall code,
   prefix_code ([::]::code) -> code = [::].
 Proof.
-  by case => [//|]; case.
+  rewrite /prefix_code.
+  case => [//|word code] /= /andP [_ /andP [/andP [H _ _]]].
+  exfalso.
+  by rewrite seqprefix_comparable0s in H.
 Qed.
 
 Inductive binary_tree :=
@@ -191,7 +255,7 @@ Proof.
   by case.
 Qed.
 
-Fixpoint tree_of_code (code: binary_code): binary_tree :=
+Fixpoint tree_of_code (code: seq binary_word): binary_tree :=
   match code with
   | nil => Empty
   | word::code' => add_word word (tree_of_code code')
@@ -229,7 +293,7 @@ Proof.
     by case: (tree_of_code code).
 Qed.
 
-Fixpoint code_of_tree (tree: binary_tree): binary_code :=
+Fixpoint code_of_tree (tree: binary_tree): seq binary_word :=
   match tree with
   | Empty => nil
   | Node l r =>
@@ -247,21 +311,44 @@ Proof.
   by case: (linear_tree word) => [//|l r ->].
 Qed.
 
-Lemma binary_code_of_binary_tree_prefix_code: forall tree,
+Lemma binary_code_code_of_tree: forall tree,
+  binary_code (code_of_tree tree).
+Proof.
+  elim => [//|l Hl r Hr /=];
+  case: ifP => [//|Hleaf].
+  move: Hr; case: (code_of_tree r) => [_ /=|word code];
+    first by rewrite cats0; apply binary_code_prepend.
+  rewrite /binary_code prepend_cons sorted_cat_cons => Hr.
+  apply /andP; split.
+  - move/sortedP in Hl.
+    apply/(sortedP [::]) => i; rewrite !nth_rcons !size_rcons !size_map.
+    case: ifP => Hi; case: ifP => Hi' Hi''.
+  -- rewrite !(nth_map [::]) => [|//|//].
+     by move/(Hl [::] i): Hi'; rewrite eqhead_lexiE.
+  -- case: ifP => [_|]; last by lia.
+     by rewrite (nth_map [::]).
+  -- by lia.
+  -- by lia.
+  - move: (binary_code_prepend true (word::code) Hr).
+    by rewrite prepend_cons.
+Qed.
+
+Lemma prefix_code_code_of_tree: forall tree,
   prefix_code (code_of_tree tree).
 Proof.
-  elim => [//|l /prefix_codeP /= [Hlu Hlc] r /prefix_codeP /= [Hru Hrc]].
+  move => tree; rewrite /prefix_code binary_code_code_of_tree /=.
+  elim: tree => [//|l Hl r Hr /=].
   case: ifP => [//|_].
-  apply /prefix_codeP; split => [|word1 word2].
-  - rewrite cat_uniq !prepend_uniq /= => [|//|//].
-    apply /andP; split => [|//].
-    by apply /negP => /hasP [word /mapP [wordl _ ->] /mapP [wordr _ []]].
-  - rewrite !mem_cat => /orP [|] /mapP [word1' H1 -> {word1}] 
-                        /orP [|] /mapP [word2' H2 -> {word2}] //;
-    rewrite seqprefix_comparable_cons => H;
-    apply f_equal.
-  -- by apply Hlc.
-  -- by apply Hrc.
+  rewrite pairwise_cat.
+  apply /andP; split;
+    first by apply /allrelP => x y /mapP [x' _ ->] /mapP [y' _ ->].
+  apply/andP; split; apply/(pairwiseP [::]) => i j;
+  rewrite !size_map => Hi Hj Hij; rewrite !(nth_map [::]) => [|//|//];
+  rewrite seqprefix_comparable_cons eq_refl /=;
+  move/(pairwiseP [::]) in Hl;
+  move/(pairwiseP [::]) in Hr.
+  - by apply Hl.
+  - by apply Hr.
 Qed.
 
 Lemma tree_of_codeK: forall tree,
@@ -276,22 +363,44 @@ Proof.
   by rewrite binary_tree_merget0.
 Qed.
 
-(* TODO(reiniscirpons): For this lemma, we need to assume that
-   code is sorted, otherwise we cannot prove it. *)
-(*Lemma code_of_treeK: forall code,*)
-(*  prefix_code code ->*)
-(*  code_of_tree (tree_of_code code) = code.*)
-(*Proof.*)
-(*  elim => [//|[|letter word] code IH];*)
-(*    first by move/prefix_code_cons_nil => ->.*)
-(*  move => /= /andP [];*)
-(*  case: letter => Hword /= /IH;*)
-(*  case: (tree_of_code code) => [<- /=|l r].*)
-(*  1,3: rewrite code_of_tree_linear_tree /=;*)
-(*       move: (linear_tree_non_empty word);*)
-(*       by case: (linear_tree word) => [//|l r _].*)
-(*  - move => /=.*)
-(*Admitted.*)
+Definition child_code (letter: bool) (code: seq binary_word):
+  seq binary_word :=
+    filter (fun x => ohead x == Some letter) code.
+
+Lemma binary_code_child_code: forall letter code,
+  binary_code code -> binary_code (child_code letter code).
+Proof.
+  move => letter code H.
+  rewrite /binary_code sorted_filter => [//||//].
+  by exact le_trans.
+Qed.
+
+Lemma prefix_code_child_code: forall letter code,
+  prefix_code code -> prefix_code (child_code letter code).
+Proof.
+  move => letter code.
+  rewrite /prefix_code => /andP [/binary_code_child_code -> /= H].
+  by apply /pairwise_filter.
+Qed.
+
+(* TODO(reiniscirpons): lemma about reconstructing binary
+   code from its children. *)
+
+Lemma code_of_treeK: forall code,
+  prefix_code code ->
+  code_of_tree (tree_of_code code) = code.
+Proof.
+  (*elim => [//|[|letter word] code IH];*)
+  (*  first by move/prefix_code_cons_nil => ->.*)
+  (*move => /=.*)
+  (*case: letter => Hword /= /IH;*)
+  (*case: (tree_of_code code) => /=.*)
+  (*=> [<- /=|l r].*)
+  (*1,3: rewrite code_of_tree_linear_tree /=;*)
+  (*     move: (linear_tree_non_empty word);*)
+  (*     by case: (linear_tree word) => [//|l r _].*)
+  (*- move => /=.*)
+Admitted.
 
 Fixpoint any_leaf (tree:binary_tree): option binary_word :=
   match tree with
@@ -323,6 +432,7 @@ Proof.
     have: (any_leaf l != None) => [|]; first by rewrite Hll.
     move => /negP /any_leaf_none; case: l {Hl Hll} => [//| ll lr /=].
 (* TODO: This sucks :( *)
+Admitted.
 
 Fixpoint follow_word (tree: binary_tree) (word: binary_word):
   option binary_word :=
@@ -373,7 +483,7 @@ Lemma follow_word_in_tree: forall tree word word',
 Proof.
   elim => [//|l Hl r Hr].
   case => [/=|].
-Qed.
+Admitted.
 
 Fixpoint complete_tree (tree: binary_tree): bool :=
   match tree with
@@ -383,12 +493,12 @@ Fixpoint complete_tree (tree: binary_tree): bool :=
     (complete_tree l && complete_tree r)
   end.
 
-Definition is_complete (P: binary_code): Prop :=
+Definition is_complete (P: seq binary_word): Prop :=
   (prefix_code P) /\
   (forall (u: binary_word), exists (v: binary_word),
    (v \in P) && (u >=< v)).
 
-Definition complete (P: binary_code): bool :=
+Definition complete (P: seq binary_word): bool :=
   (prefix_code P) && (complete_tree (tree_of_code P)).
 
 Lemma completeP: forall P,
@@ -398,6 +508,4 @@ Proof.
   - case => HP Htree; split => [//|u].
     pose v := (follow_word (tree_of_code P) u).
 Admitted.
-
-
 
